imper/InOut.ml
@@ -7,24 +7,5 @@ let std_dup_sum () =
       print_int x;
       s := !s + x;
    done;
-   print_int s
+   print_int !s
 
-(*
-
-Parameter Channel : forall (L:list dyn) (l:loc), hprop.
-
-Notation "l ~>> L" := (l ~> Channel L)
-  (at level 32, no associativity).
-
-Spec ml_read_int () |R>> forall L,
-  R (stdin ~>> n::L) (||=n|| \*+ stdin ~>> L)
-
-Spec ml_print_int n |R>> forall L,
-  R (stdout ~>> L) (# stdout ~>> L & n)
-
-Spec std_dup_sum () |R>> forall n L Li Lo,  
-  n = length L ->
-  R (stdin ~>> Channel n::L++Li \* stdout ~>> Lo)
-    (# stdin ~>> Li \* stdout ~>> Lo ++ L & (fold plus 0 L))
-
-*)
