imper/InOut_proof.v
@@ -1,19 +1,62 @@
-(*
+Set Implicit Arguments.
+Require Import CFPrim InOut_ml.
 
-Parameter Channel : forall (L:list dyn) (l:loc), hprop.
 
-Notation "l ~>> L" := (l ~> Channel L)
-  (at level 32, no associativity).
+Ltac xfor_base_manual I cont1 cont2 := 
+  apply local_erase; split; 
+    [ cont1 tt 
+    | cont2 tt; esplit; exists I; splits 3%nat; 
+       [  
+       | xfor_bounds_intro tt
+       | ]
+    ].
 
-Spec ml_read_int () |R>> forall L,
-  R (stdin ~>> n::L) (||=n|| \*+ stdin ~>> L)
+Ltac xfor_core_gen_manual I H :=
+  xfor_base_manual I ltac:(fun _ => intros H)
+                     ltac:(fun _ => intros H).
 
-Spec ml_print_int n |R>> forall L,
-  R (stdout ~>> L) (# stdout ~>> L & n)
+Ltac xfor_base_gen_manual I H :=
+  xfor_pre ltac:(fun _ => xfor_core_gen_manual I H).
 
-Spec std_dup_sum () |R>> forall n L Li Lo,  
+Tactic Notation "xfor_general_manual" constr(I) "as" ident(H) := 
+  xfor_base_gen_manual I H.
+Tactic Notation "xfor_general_manual" constr(I) := 
+  let H := fresh "Hfor" in xfor_general_manual I as H.
+
+
+(********************************************************************)
+
+Implicit Arguments dyn [[dyn_type]].
+
+Definition list_dyn A (L:list A) :=
+  LibList.map dyn L.
+
+Lemma std_dup_sum_spec :
+  Spec std_dup_sum () |R>> forall (n:int) (L:list int) Li Lo,  
   n = length L ->
-  R (stdin ~>> Channel n::L++Li \* stdout ~>> Lo)
-    (# stdin ~>> Li \* stdout ~>> Lo ++ L & (fold plus 0 L))
+  R (stdin ~>> (dyn n :: list_dyn L ++ Li) \* stdout ~>> Lo)
+    (# stdin ~>> Li \* stdout ~>> (Lo ++ list_dyn L & dyn (fold_left Zplus 0 L))).
+Proof.
+  xcf. introv E.
+  xapp. intro_subst.
+  xapp.
+  xfor_general_manual (fun i => 
+    Hexists (S:int), Hexists L1 L2, 
+      [i = 1+length L1 /\ L = L1 ++ L2 /\ S = fold_left Zplus 0 L1] \*
+      s ~> Ref Id S \* stdin ~>> (list_dyn L2 ++ Li) \* stdout ~>> (Lo ++ list_dyn L1)).
+    skip. (* todo: case no exec *)
+    (* forwards N: (@length_zero_inv _ L). math. subst L. rew_length in E. subst n. *)
+    (* loop start *)
+    hsimpl (0%Z) (@nil int) L.
+      unfold list_dyn. rew_list~.
+      splits. rew_length. math. auto. auto.
+    (* loop body *)
+    
+    (* loop end *)
+  
 
-*)
+
+  
+
+Qed.
+
